\documentclass[fleqn]{article}
\setlength{\topmargin}{0in} \setlength{\oddsidemargin}{0in}
\setlength{\evensidemargin}{0in} \setlength{\headheight}{0in}
\setlength{\headsep}{0in} \setlength{\textwidth}{6.5in}
\setlength{\textheight}{9in}
\setlength{\mathindent}{0pt}

\usepackage[fleqn]{amsmath}
\usepackage{dsfont}
\usepackage{graphicx}
\usepackage{url}
%\usepackage{chicago}
\usepackage{natbib}
\def\bm#1{\mbox{\boldmath $#1$}}
 
\title{Spatial Geostatistical Model}
\author{John Tipton}
\date{\today}
\begin{document}
\maketitle

\section{Full Dimensional Model Statement}
%
\subsection{Data Model}
\begin{align*}
\bm{y}_t & = \bm{H}_t \bm{X} \bm{\beta}_t + \bm{\eta}_t + \bm{\epsilon}_t\\
%
\end{align*}
%
\subsection{Process Model}
%
\begin{align*}
%
% \bm{\beta}_t & \sim N(\bm{\mu}_\beta, \bm{\Sigma}_\beta) & \bm{\Sigma}_\beta &  = \sigma^2_\epsilon \bm{D}_\gamma & \bm{D}_\gamma & = diag(\gamma^2_1, \ldots, \gamma^2_\tau)\\
\bm{\beta}_t & \sim N(\bm{0}, \bm{\Sigma}_\beta) & \bm{\Sigma}_\beta &  = \sigma^2_\epsilon \bm{D}_\gamma & \bm{D}_\gamma & = diag(\gamma^2_1, \ldots, \gamma^2_\tau)\\
%
\bm{\eta}_t & \sim N(0, \bm{\Sigma}_{\eta_t}) & \bm{\Sigma}_{\eta_t} &  = \sigma^2_\eta \bm{R}_t(\phi) & \bm{R}_t(\phi) & = \exp{( - \bm{D}_t / \phi)}\\
%
\bm{\epsilon}_t & \sim N(0, \bm{\Sigma}_{\epsilon_t}) & \bm{\Sigma}_{\epsilon_t} &  = \sigma^2_\epsilon \bm{I}_{n_t}\\
%
\bm{\gamma^2_i} & \sim Exp(\lambda^2 / 2) \mbox{ Equivalently} & \frac{1} {\gamma^2_i} & \sim IG(1, \lambda^2 / 2) & &  \mbox{for } i =1 \ldots, \tau\\
%
\end{align*}
%
\subsection{Parameter Model}
%
\begin{align*}
%
% \bm{\mu}_\beta & \sim N(\bm{\mu}_0, \bm{\Sigma}_0)\\
%
% \sigma^2_\beta & \sim IG(\alpha_\beta, \beta_\beta)\\
%
\sigma^2_\eta & \sim IG(\alpha_\eta, \beta_\eta)\\
%
\sigma^2_\epsilon & \sim IG(\alpha_\epsilon, \beta_\epsilon)\\
%
\phi & \sim IG(\alpha_\phi, \beta_\phi)\\
%
\lambda^2 & \sim \Gamma(\alpha_\lambda, \beta_\lambda)\\
\end{align*}
%
where $\bm{I}_{n_t}$ is the identity matrix of size $n_t \times n_t$ where $\tau$ is the number of parameters in $\bm{\beta}_t$ and $n_t$ is the number of samples of $y_t$ at time $t$ and $\bm{D}_t$ is the distance matrix between locations observed at time $t$. Define $\bm{\Sigma}_t = \bm{\Sigma}_{\eta_t} + \bm{\Sigma}_{\epsilon_t}$
%
\section{Posterior}
%
\begin{align*}
\prod_{t = 1}^T [\bm{\beta}_t, \bm{\gamma}^2, \sigma^2_\eta, \sigma^2_\epsilon, \phi, \lambda^2 | \bm{y}_t] & \propto \prod_{t = 1}^T [\bm{y}_t | \bm{\beta}_t, \sigma^2_\eta, \phi, \sigma^2_\epsilon] [\bm{\beta}_t | \sigma^2_\epsilon, \bm{\gamma^2}] [\bm{\gamma} | \lambda^2] [\sigma^2_\eta] [\sigma^2_\epsilon] [\phi] [\lambda^2]
\end{align*}
%
\section{Full Conditionals}
%
\subsection{Full Conditional for $\bm{\beta}_t$}
%
For $t = 1, \ldots, T$,
\begin{align*}
[\bm{\beta}_t | \cdot] & \propto [\bm{y}_t | \bm{\beta}_t, \sigma^2_\eta, \sigma^2_\epsilon, \phi] [\bm{\beta}_t | \bm{\mu}_\beta, \sigma^2_\beta]\\
%
& \propto e^{ - \frac{1} {2} (\bm{y}_t - \bm{H}_t \bm{X} \bm{\beta}_t)^T \bm{\Sigma}_t^{ - 1} (\bm{y}_t - \bm{H}_t \bm{X} \bm{\beta}_t)} e^{ - \frac{1} {2} \bm{\beta}_t^T \bm{\Sigma}_\beta^{ - 1} \bm{\beta}_t}\\
%
& \propto e^{ - \frac{1} {2} \{\bm{\beta}_t^T (\bm{X}^T \bm{H}_t^T \bm{\Sigma}_t^{ - 1} \bm{H}_t \bm{X} + \bm{\Sigma}_\beta^{ - 1}) \bm{\beta}_t - 2 \bm{\beta}_t^T (\bm{X}^T \bm{H}_t^T \bm{\Sigma}_t^{ - 1} \bm{y}_t) \} }
\end{align*}
%
which is Normal with mean $ \bm{A}^{ - 1} \bm{b}$ and variance $\bm{A}^{ - 1}$ where
\begin{align*}
  \bm{A}^{ - 1} & = (\bm{X}^T \bm{H}_t^T \bm{\Sigma}_t^{ - 1} \bm{H}_t \bm{X} + \bm{\Sigma}_\beta^{ - 1})^{ - 1}\\
  %
  \bm{b} & = (\bm{X}^T \bm{H}_t^T \bm{\Sigma}_t^{ - 1} \bm{y}_t)\\
\end{align*}
%
% \subsection{Full Conditional for $\bm{\mu}_\beta$}
% %
% \begin{align*}
% [\bm{\mu}_\beta | \cdot] & \propto \prod_{t = 1}^T [\bm{\beta}_t | \bm{\mu}_\beta, \sigma^2_\beta] [\bm{\mu}_\beta]\\
% %
% & \propto e^{ - \frac{1} {2} \sum_{t = 1}^T (\bm{\beta}_t - \bm{\mu}_\beta)^T \bm{\Sigma}_\beta^{ - 1} (\bm{\beta}_t - \bm{\mu}_\beta)} e^{ - \frac{1} {2} (\bm{\mu}_\beta - \bm{\mu}_0)^T \Sigma_0^{ - 1} (\bm{\mu}_\beta - \bm{\mu}_0)}\\
% %
% & \propto e^{ - \frac{1} {2} (
% \bm{\mu}_\beta^T (T \bm{\Sigma}_\beta^{ - 1} + \bm{\Sigma}_0^{ - 1}) \bm{\mu}_\beta - 2 \bm{\mu}_\beta^T (\sum_{t = 1}^T \bm{\Sigma}_\beta^{ - 1} \bm{\beta}_t + \bm{\Sigma}_0^{ - 1} \bm{\mu}_0) ) }
% \end{align*}
% %
% which is multivariate normal with mean
% $(T \bm{\Sigma}_\beta^{ - 1} + \bm{\Sigma}_0^{ - 1})^{ - 1} (\sum_{t = 1}^T \bm{\Sigma}_\beta^{ - 1} \bm{\beta}_t + \bm{\Sigma}_0^{ - 1} \bm{\mu}_0)$ and variance $(T \bm{\Sigma}_\beta^{ - 1} + \bm{\Sigma}_0^{ - 1})^{ - 1}$
%
% \subsection{Full Conditional for $\sigma^2_\beta$}
% %
% \begin{align*}
% [\sigma^2_\beta | \cdot] & \propto \prod_{t = 1}^T [\bm{\beta}_t | \bm{\mu}_\beta, \sigma^2_\beta] [\sigma^2_\beta]\\
% %
% & \propto (\prod_{t = 1}^T |\bm{\Sigma}_\beta|^{ - \frac{1} {2}}) e^{ - \frac{1} {2} \sum_{t = 1}^T (\bm{\beta}_t - \bm{\mu}_\beta)^T \bm{\Sigma}_\beta^{ - 1} (\bm{\beta}_t - \bm{\mu}_\beta)} (\sigma^2_\beta)^{ - (\alpha_\beta + 1)} e^{ - \frac{\beta_\beta} {\sigma^2_\beta}}\\
% %
% & \propto (\sigma^2_\beta)^{ - (\alpha_\beta + \frac{\sum_{t = 1}^T n_t} {2} + 1)} e^{ - \frac{1} {\sigma^2_\beta} (\frac{1} {2} \sum_{t = 1}^T (\bm{\beta}_t - \bm{\mu}_\beta)^T (\bm{\beta}_t - \bm{\mu}_\beta) + \beta_\beta)}
% \end{align*}
% %
% which is IG$(\alpha_\beta + \frac{\sum_{t = 1}^T n_t} {2}, \frac{1} {2} \sum_{t = 1}^T (\bm{\beta}_t - \bm{\mu}_\beta)^T (\bm{\beta}_t - \bm{\mu}_\beta) + \beta_\beta)$ since the determinant $|\bm{\Sigma}_\beta| = (\sigma^2_\beta)^{n_t}$ and $\bm{\Sigma}_\beta^{ - 1} = \frac{1} {\sigma^2_\beta} \bm{I}_t$
%
%
% \subsection{Full Conditional for $\gamma^2_i$}
% For $i = 1, \ldots, \tau$
% \begin{align*}
% [\gamma^2_i | \cdot] & \propto \prod_{t = 1}^T [\beta_t | \sigma^2_\epsilon, \gamma^2_i] [\gamma^2_i | \lambda^2]\\
%  %
%  & \propto \prod_{t = 1}^T |\sigma^2_\epsilon \gamma^2_i|^{ - \frac{1} {2}} e^{ - \frac{1} {2} \beta_t^T (\sigma^2_\epsilon \gamma^2_i)^{ - 1} \beta_t} (\frac{1} {\gamma^2_i})^{ - 2} e^{-\frac{\lambda^2 / 2} {\frac{1} {\gamma^2_i}}}\\
% %
% & \propto (\gamma^2_i)^{ - \frac{T} {2}} e^{ - \frac{1} {\gamma^2_i}(\frac{\sum_{t = 1}^T \beta_t^T \beta_t} {2 \sigma^2_\epsilon})} (\gamma^2_i)^{2} e^{ - \frac{\lambda^2 / 2} {\frac{1} {\gamma^2_i}}}\\
% %
% & \propto (\frac{1} {\gamma^2_i})^{2 - \frac{T} {2}} e^{ - \frac{1} {\gamma^2_i}(\frac{\sum_{t = 1}^T \beta_t^T \beta_t} {2 \sigma^2_\epsilon})} (\frac{1} {\gamma^2_i})^{ - 2} e^{ - \frac{\lambda^2 / 2} {\frac{1} {\gamma^2_i}}}
% \end{align*}
% 
% NEED TO WORK ON THIS ONE SOME MORE!!
% !!!
% !!
\subsection{Full Conditional for $\gamma^2_i$}
For $i = 1, \ldots, \tau$
\begin{align*}
[\gamma^2_i | \cdot] & \propto \prod_{t = 1}^T [\beta_t | \sigma^2_\epsilon, \gamma^2_i] [\gamma^2_i | \lambda^2]\\
 %
 & \propto \prod_{t = 1}^T |\sigma^2_\epsilon \gamma^2_i|^{ - \frac{1} {2}} e^{ - \frac{1} {2} \beta_t^T (\sigma^2_\epsilon \gamma^2_i)^{ - 1} \beta_t} e^{-\frac{\lambda^2} {2} \gamma^2_i}\\
%
& \propto (\gamma^2_i)^{ - \frac{T} {2}} e^{ - \frac{1} {\gamma^2_i}(\frac{\sum_{t = 1}^T \beta_t^T \beta_t} {2 \sigma^2_\epsilon})} e^{ - \frac{\lambda^2} {2} \gamma^2_i}\\
%
\end{align*}


\subsection{Full Conditional for $\sigma^2_\eta$}
%
\begin{align*}
[\sigma^2_\eta | \cdot] & \propto \prod_{t = 1}^T [\bm{y}_t | \bm{\beta}_t, \sigma^2_\eta, \phi, \sigma^2_\epsilon] [\sigma^2_\eta]\\
%
& \propto (\prod_{t = 1}^T |\bm{\Sigma}_t |^{ - \frac{1} {2}}) e^{ - \frac{1} {2} \sum_{t = 1}^T (\bm{y}_t - \bm{H}_t \bm{X} \bm{\beta}_t)^T \bm{\Sigma}_t^{ - 1} (\bm{y}_t - \bm{H}_t \bm{X} \bm{\beta}_t)} (\sigma^2_\eta)^{ - \alpha_\eta - 1} e^{ - \frac{\beta_\eta} {\sigma^2_\eta}}\\
%
& \propto |\bm{\Sigma}_t |^{ - \frac{T} {2}} e^{ - \frac{1} {2} \sum_{t = 1}^T (\bm{y}_t - \bm{H}_t \bm{X} \bm{\beta}_t)^T \bm{\Sigma}_t^{ - 1} (\bm{y}_t - \bm{H}_t \bm{X} \bm{\beta}_t)} (\sigma^2_\eta)^{ - \alpha_\eta - 1} e^{ - \frac{\beta_\eta} {\sigma^2_\eta}}\\
\end{align*}
% 
which can be sampled using a Metropolis-Hastings step
%
\subsection{Full Conditional for $\sigma^2_\epsilon$}
%
\begin{align*}
[\sigma^2_\epsilon | \cdot] & \propto \prod_{t = 1}^T [\bm{y}_t | \bm{\beta}_t, \sigma^2_\eta, \phi, \sigma^2_\epsilon] [\bm{\beta}_t | \sigma^2_\eta, \bm{\gamma}] [\sigma^2_\epsilon]\\
%
& \propto (\prod_{t = 1}^T |\bm{\Sigma}_t |^{ - \frac{1} {2}}) e^{ - \frac{1} {2} \sum_{t = 1}^T (\bm{y}_t - \bm{H}_t \bm{X} \bm{\beta}_t)^T \bm{\Sigma}_t^{ - 1} (\bm{y}_t - \bm{H}_t \bm{X} \bm{\beta}_t)} |\bm{\Sigma}_\beta |^{ - \frac{1} {2}} e^{ - \frac{1} {2} \sum_{t = 1}^T \bm{\beta}_t^T \bm{\Sigma}_{\beta}^{ - 1} \bm{\beta}_t} (\sigma^2_\epsilon)^{ - \alpha_\epsilon - 1} e^{ - \frac{\beta_\epsilon} {\sigma^2_\epsilon}}\\
%
& \propto |\bm{\Sigma}_t |^{ - \frac{T} {2}} e^{ - \frac{1} {2} \sum_{t = 1}^T (\bm{y}_t - \bm{H}_t \bm{X} \bm{\beta}_t)^T \bm{\Sigma}_t^{ - 1} (\bm{y}_t - \bm{H}_t \bm{X} \bm{\beta}_t)} |\bm{\Sigma}_\beta |^{ - \frac{1} {2}} e^{ - \frac{1} {2} \sum_{t = 1}^T \bm{\beta}_t^T \bm{\Sigma}_{\beta}^{ - 1} \bm{\beta}_t} (\sigma^2_\epsilon)^{ - \alpha_\epsilon - 1} e^{ - \frac{\beta_\epsilon} {\sigma^2_\epsilon}}\\
\end{align*}
% 
which can be sampled using a Metropolis-Hastings step
%
\subsection{Full Conditional for $\phi$}
%
\begin{align*}
  [\phi | \cdot] & \propto \prod_{t = 1}^T [y_t | \beta_t, \sigma^2_\eta, \phi, \sigma^2_\epsilon] [\phi]\\
%
& \propto \prod_{t = 1}^T | \bm{\Sigma}_t |^{ - \frac{1} {2}} e^{ - \frac{1} {2} (\bm{y}_t - \bm{H}_t \bm{X} \bm{\beta}_t)^T \bm{\Sigma}_t^{ - 1} (\bm{y}_t - \bm{H}_t \bm{X} \bm{\beta}_t)} \phi^{ - \alpha_\phi - 1} e^{ - \frac{\beta_\phi} {\phi}}\\
%
& \propto | \bm{\Sigma}_t |^{ - \frac{T} {2}} e^{ - \frac{1} {2} \sum_{t = 1}^T (\bm{y}_t - \bm{H}_t \bm{X} \bm{\beta}_t)^T \bm{\Sigma}_t^{ - 1} (\bm{y}_t - \bm{H}_t \bm{X} \bm{\beta}_t)} \phi^{ - \alpha_\phi - 1} e^{ - \frac{\beta_\phi} {\phi}}\\
\end{align*}
% 
which can be sampled using a Metropolis-Hastings step
%
\subsection*{Full Conditional for $\lambda^2$}
%
\begin{align*}
[\lambda^2 | \cdot] & \propto \prod_{t = 1}^T \prod_{j = 1}^\tau (\lambda^2) e^{ - \frac{\lambda^2 / 2} {1 / \gamma^2_j}} (\frac{\lambda^2} {2})^{\alpha_\lambda - 1} e^{ - \beta_\lambda (\lambda^2 /2)}\\
%
& \propto (\frac{\lambda^2} {2})^{\alpha_\lambda + \tau - 1} e^{ - \lambda^2(\beta_\lambda + \sum_{j = 1}^\tau \gamma^2_j / 2)}
\end{align*}
%
which is Gamma($\alpha_\lambda + \tau, \beta_\lambda + \sum_{j = 1}^\tau \gamma^2_j / 2$)
%
\section{Posterior Predictive Distribution}
%
The posterior predictive distribution for $\bm{y}_t$ is sampled a each MCMC iteration $k$ by
\begin{align*}
  \bm{y}^{(k)}_t & \sim N(\bm{H_t} \bm{X} \bm{\beta}^{(k)}_t, \bm{\Sigma}^{(k)})
\end{align*}


\end{document}
